AVATAR_executablecode/generated_src/EDRSystemBlock.c
@@ -17,193 +17,205 @@
 #define STATE__ParseIndicatorState 14
 #define STATE__STOP__STATE 15
 
-void *mainFunc__EDRSystemBlock(void *arg){
-  can_frame canFrame;
-  uint32_t canID;
-  uint8_t canDLC;
-  uint8_t* data;
-  fstar_uint8_array speed;
-  fstar_uint8 indicator;
-  fstar_uint8 door;
-  uint32_t code;
-  uint8_t* message;
-  int32_t recordInEDRResult;
-  int32_t fd;
-  int64_t timestamp;
-  
-  int __currentState = STATE__START__STATE;
-  
-  char * __myname = (char *)arg;
-  
-  pthread_cond_init(&__myCond__EDRSystemBlock, NULL);
-  
-  fillListOfRequests(&__list__EDRSystemBlock, __myname, &__myCond__EDRSystemBlock, &__mainMutex);
-  //printf("my name = %s\n", __myname);
-  
-  /* Main loop on states */
-  while(__currentState != STATE__STOP__STATE) {
-    switch(__currentState) {
-      case STATE__START__STATE: 
-      __currentState = STATE__EDRSystemStartState;
-      break;
-      
-      case STATE__EDRSystemStartState: 
-      fd = getSocket();
-      __currentState = STATE__PacketCaptureState;
-      break;
-      
-      case STATE__PacketCaptureState: 
-      canFrame = packetCapture(fd);
-      canID = canFrame.can_id;
-      canDLC = canFrame.can_dlc;
-      data = canFrame.data;
-      timestamp = canFrame.timestamp;
-      __currentState = STATE__PacketParseState;
-      break;
-      
-      case STATE__PacketParseState: 
-      if (canID == 0x1b4) {
-        makeNewRequest(&__req0__EDRSystemBlock, 105, IMMEDIATE, 0, 0, 0, 0, __params0__EDRSystemBlock);
-        addRequestToList(&__list__EDRSystemBlock, &__req0__EDRSystemBlock);
-      }
-      if (canID == 0x188) {
-        makeNewRequest(&__req1__EDRSystemBlock, 109, IMMEDIATE, 0, 0, 0, 0, __params1__EDRSystemBlock);
-        addRequestToList(&__list__EDRSystemBlock, &__req1__EDRSystemBlock);
-      }
-      if (canID == 0x19b) {
-        makeNewRequest(&__req2__EDRSystemBlock, 113, IMMEDIATE, 0, 0, 0, 0, __params2__EDRSystemBlock);
-        addRequestToList(&__list__EDRSystemBlock, &__req2__EDRSystemBlock);
-      }
-      if (nbOfRequests(&__list__EDRSystemBlock) == 0) {
-        debug2Msg(__myname, "No possible request");
-        __currentState = STATE__STOP__STATE;
-        break;
-      }
-      __returnRequest__EDRSystemBlock = executeListOfRequests(&__list__EDRSystemBlock);
-      clearListOfRequests(&__list__EDRSystemBlock);
-       if (__returnRequest__EDRSystemBlock == &__req0__EDRSystemBlock) {
-        __currentState = STATE__ParseSpeedState;
-        
-      }
-      else  if (__returnRequest__EDRSystemBlock == &__req1__EDRSystemBlock) {
-        __currentState = STATE__ParseIndicatorState;
-        
-      }
-      else  if (__returnRequest__EDRSystemBlock == &__req2__EDRSystemBlock) {
-        __currentState = STATE__ParseDoorState;
-        
-      }
-      break;
-      
-      case STATE__ParseSpeedState: 
-      speed = parseSpeed(canID, canDLC, data);
-      code = speed.struct_error.code;
-      message = speed.struct_error.message;
-      __currentState = STATE__CheckValidationResultState;
-      break;
-      
-      case STATE__CheckValidationResultState: 
-      if (code == 0) {
-        makeNewRequest(&__req0__EDRSystemBlock, 167, IMMEDIATE, 0, 0, 0, 0, __params0__EDRSystemBlock);
-        addRequestToList(&__list__EDRSystemBlock, &__req0__EDRSystemBlock);
-      }
-      if (code > 0) {
-        makeNewRequest(&__req1__EDRSystemBlock, 170, IMMEDIATE, 0, 0, 0, 0, __params1__EDRSystemBlock);
-        addRequestToList(&__list__EDRSystemBlock, &__req1__EDRSystemBlock);
-      }
-      if (nbOfRequests(&__list__EDRSystemBlock) == 0) {
-        debug2Msg(__myname, "No possible request");
-        __currentState = STATE__STOP__STATE;
-        break;
-      }
-      __returnRequest__EDRSystemBlock = executeListOfRequests(&__list__EDRSystemBlock);
-      clearListOfRequests(&__list__EDRSystemBlock);
-       if (__returnRequest__EDRSystemBlock == &__req0__EDRSystemBlock) {
-        __currentState = STATE__RecordInEDRState;
-        
-      }
-      else  if (__returnRequest__EDRSystemBlock == &__req1__EDRSystemBlock) {
-        __currentState = STATE__ValidationErrorState;
-        
-      }
-      break;
-      
-      case STATE__RecordInEDRState: 
-      recordInEDRResult = record_in_edr(canID, timestamp, speed, indicator, door);
-      __currentState = STATE__CheckRecordInEDRResultState;
-      break;
-      
-      case STATE__CheckRecordInEDRResultState: 
-      if (recordInEDRResult == 0) {
-        makeNewRequest(&__req0__EDRSystemBlock, 82, IMMEDIATE, 0, 0, 0, 0, __params0__EDRSystemBlock);
-        addRequestToList(&__list__EDRSystemBlock, &__req0__EDRSystemBlock);
-      }
-      if (recordInEDRResult == 1) {
-        makeNewRequest(&__req1__EDRSystemBlock, 87, IMMEDIATE, 0, 0, 0, 0, __params1__EDRSystemBlock);
-        addRequestToList(&__list__EDRSystemBlock, &__req1__EDRSystemBlock);
-      }
-      if (recordInEDRResult == 2) {
-        makeNewRequest(&__req2__EDRSystemBlock, 91, IMMEDIATE, 0, 0, 0, 0, __params2__EDRSystemBlock);
-        addRequestToList(&__list__EDRSystemBlock, &__req2__EDRSystemBlock);
-      }
-      if (nbOfRequests(&__list__EDRSystemBlock) == 0) {
-        debug2Msg(__myname, "No possible request");
-        __currentState = STATE__STOP__STATE;
-        break;
-      }
-      __returnRequest__EDRSystemBlock = executeListOfRequests(&__list__EDRSystemBlock);
-      clearListOfRequests(&__list__EDRSystemBlock);
-       if (__returnRequest__EDRSystemBlock == &__req0__EDRSystemBlock) {
-        __currentState = STATE__NormalLoopState;
-        
-      }
-      else  if (__returnRequest__EDRSystemBlock == &__req1__EDRSystemBlock) {
-        __currentState = STATE__WroteEventToRecordState;
-        
-      }
-      else  if (__returnRequest__EDRSystemBlock == &__req2__EDRSystemBlock) {
-        __currentState = STATE__EDRErrorState;
-        
-      }
-      break;
-      
-      case STATE__WroteEventToRecordState: 
-      __currentState = STATE__EDRSystemEndState;
-      break;
-      
-      case STATE__EDRSystemEndState: 
-      __currentState = STATE__STOP__STATE;
-      break;
-      
-      case STATE__EDRErrorState: 
-      __currentState = STATE__PacketCaptureState;
-      break;
-      
-      case STATE__NormalLoopState: 
-      __currentState = STATE__PacketCaptureState;
-      break;
-      
-      case STATE__ValidationErrorState: 
-      __currentState = STATE__PacketCaptureState;
-      break;
-      
-      case STATE__ParseDoorState: 
-      door = parseDoor(canID, canDLC, data);
-      code = door.struct_error.code;
-      message = door.struct_error.message;
-      __currentState = STATE__CheckValidationResultState;
-      break;
-      
-      case STATE__ParseIndicatorState: 
-      indicator = parseIndicator(canID, canDLC, data);
-      code = indicator.struct_error.code;
-      message = indicator.struct_error.message;
-      __currentState = STATE__CheckValidationResultState;
-      break;
-      
-    }
-  }
-  //printf("Exiting = %s\n", __myname);
-  return NULL;
-}
+void *mainFunc__EDRSystemBlock(void *arg)
+{
+    can_frame canFrame;
+    uint32_t canID;
+    uint8_t canDLC;
+    uint8_t *data;
+    fstar_uint8_array speed;
+    fstar_uint8 indicator;
+    fstar_uint8 door;
+    uint32_t code;
+    C_String_t message;
+    int32_t recordInEDRResult;
+    int32_t fd;
+    int64_t timestamp;
 
+    int __currentState = STATE__START__STATE;
+
+    char *__myname = (char *)arg;
+
+    pthread_cond_init(&__myCond__EDRSystemBlock, NULL);
+
+    fillListOfRequests(&__list__EDRSystemBlock, __myname, &__myCond__EDRSystemBlock, &__mainMutex);
+    // printf("my name = %s\n", __myname);
+
+    /* Main loop on states */
+    while (__currentState != STATE__STOP__STATE)
+    {
+        switch (__currentState)
+        {
+        case STATE__START__STATE:
+            __currentState = STATE__EDRSystemStartState;
+            break;
+
+        case STATE__EDRSystemStartState:
+            fd = getSocket();
+            __currentState = STATE__PacketCaptureState;
+            break;
+
+        case STATE__PacketCaptureState:
+            canFrame = packetCapture(fd);
+            canID = canFrame.can_id;
+            canDLC = canFrame.can_dlc;
+            data = canFrame.data;
+            timestamp = canFrame.timestamp;
+            __currentState = STATE__PacketParseState;
+            break;
+
+        case STATE__PacketParseState:
+            if (canID == 0x1b4)
+            {
+                makeNewRequest(&__req0__EDRSystemBlock, 278, IMMEDIATE, 0, 0, 0, 0, __params0__EDRSystemBlock);
+                addRequestToList(&__list__EDRSystemBlock, &__req0__EDRSystemBlock);
+            }
+            if (canID == 0x188)
+            {
+                makeNewRequest(&__req1__EDRSystemBlock, 282, IMMEDIATE, 0, 0, 0, 0, __params1__EDRSystemBlock);
+                addRequestToList(&__list__EDRSystemBlock, &__req1__EDRSystemBlock);
+            }
+            if (canID == 0x19b)
+            {
+                makeNewRequest(&__req2__EDRSystemBlock, 286, IMMEDIATE, 0, 0, 0, 0, __params2__EDRSystemBlock);
+                addRequestToList(&__list__EDRSystemBlock, &__req2__EDRSystemBlock);
+            }
+            if (nbOfRequests(&__list__EDRSystemBlock) == 0)
+            {
+                debug2Msg(__myname, "No possible request");
+                __currentState = STATE__STOP__STATE;
+                break;
+            }
+            __returnRequest__EDRSystemBlock = executeListOfRequests(&__list__EDRSystemBlock);
+            clearListOfRequests(&__list__EDRSystemBlock);
+            if (__returnRequest__EDRSystemBlock == &__req0__EDRSystemBlock)
+            {
+                __currentState = STATE__ParseSpeedState;
+            }
+            else if (__returnRequest__EDRSystemBlock == &__req1__EDRSystemBlock)
+            {
+                __currentState = STATE__ParseIndicatorState;
+            }
+            else if (__returnRequest__EDRSystemBlock == &__req2__EDRSystemBlock)
+            {
+                __currentState = STATE__ParseDoorState;
+            }
+            break;
+
+        case STATE__ParseSpeedState:
+            speed = parseSpeed(canID, canDLC, data);
+            code = speed.error.code;
+            message = speed.error.message;
+            __currentState = STATE__CheckValidationResultState;
+            break;
+
+        case STATE__CheckValidationResultState:
+            if (code == 0)
+            {
+                makeNewRequest(&__req0__EDRSystemBlock, 340, IMMEDIATE, 0, 0, 0, 0, __params0__EDRSystemBlock);
+                addRequestToList(&__list__EDRSystemBlock, &__req0__EDRSystemBlock);
+            }
+            if (code > 0)
+            {
+                makeNewRequest(&__req1__EDRSystemBlock, 343, IMMEDIATE, 0, 0, 0, 0, __params1__EDRSystemBlock);
+                addRequestToList(&__list__EDRSystemBlock, &__req1__EDRSystemBlock);
+            }
+            if (nbOfRequests(&__list__EDRSystemBlock) == 0)
+            {
+                debug2Msg(__myname, "No possible request");
+                __currentState = STATE__STOP__STATE;
+                break;
+            }
+            __returnRequest__EDRSystemBlock = executeListOfRequests(&__list__EDRSystemBlock);
+            clearListOfRequests(&__list__EDRSystemBlock);
+            if (__returnRequest__EDRSystemBlock == &__req0__EDRSystemBlock)
+            {
+                __currentState = STATE__RecordInEDRState;
+            }
+            else if (__returnRequest__EDRSystemBlock == &__req1__EDRSystemBlock)
+            {
+                __currentState = STATE__ValidationErrorState;
+            }
+            break;
+
+        case STATE__RecordInEDRState:
+            recordInEDRResult = record_in_edr(canID, timestamp, speed, indicator, door);
+            __currentState = STATE__CheckRecordInEDRResultState;
+            break;
+
+        case STATE__CheckRecordInEDRResultState:
+            if (recordInEDRResult == 0)
+            {
+                makeNewRequest(&__req0__EDRSystemBlock, 255, IMMEDIATE, 0, 0, 0, 0, __params0__EDRSystemBlock);
+                addRequestToList(&__list__EDRSystemBlock, &__req0__EDRSystemBlock);
+            }
+            if (recordInEDRResult == 1)
+            {
+                makeNewRequest(&__req1__EDRSystemBlock, 260, IMMEDIATE, 0, 0, 0, 0, __params1__EDRSystemBlock);
+                addRequestToList(&__list__EDRSystemBlock, &__req1__EDRSystemBlock);
+            }
+            if (recordInEDRResult == 2)
+            {
+                makeNewRequest(&__req2__EDRSystemBlock, 264, IMMEDIATE, 0, 0, 0, 0, __params2__EDRSystemBlock);
+                addRequestToList(&__list__EDRSystemBlock, &__req2__EDRSystemBlock);
+            }
+            if (nbOfRequests(&__list__EDRSystemBlock) == 0)
+            {
+                debug2Msg(__myname, "No possible request");
+                __currentState = STATE__STOP__STATE;
+                break;
+            }
+            __returnRequest__EDRSystemBlock = executeListOfRequests(&__list__EDRSystemBlock);
+            clearListOfRequests(&__list__EDRSystemBlock);
+            if (__returnRequest__EDRSystemBlock == &__req0__EDRSystemBlock)
+            {
+                __currentState = STATE__NormalLoopState;
+            }
+            else if (__returnRequest__EDRSystemBlock == &__req1__EDRSystemBlock)
+            {
+                __currentState = STATE__WroteEventToRecordState;
+            }
+            else if (__returnRequest__EDRSystemBlock == &__req2__EDRSystemBlock)
+            {
+                __currentState = STATE__EDRErrorState;
+            }
+            break;
+
+        case STATE__WroteEventToRecordState:
+            __currentState = STATE__EDRSystemEndState;
+            break;
+
+        case STATE__EDRSystemEndState:
+            __currentState = STATE__STOP__STATE;
+            break;
+
+        case STATE__EDRErrorState:
+            __currentState = STATE__PacketCaptureState;
+            break;
+
+        case STATE__NormalLoopState:
+            __currentState = STATE__PacketCaptureState;
+            break;
+
+        case STATE__ValidationErrorState:
+            __currentState = STATE__PacketCaptureState;
+            break;
+
+        case STATE__ParseDoorState:
+            door = parseDoor(canID, canDLC, data);
+            code = door.error.code;
+            message = door.error.message;
+            __currentState = STATE__CheckValidationResultState;
+            break;
+
+        case STATE__ParseIndicatorState:
+            indicator = parseIndicator(canID, canDLC, data);
+            code = indicator.error.code;
+            message = indicator.error.message;
+            __currentState = STATE__CheckValidationResultState;
+            break;
+        }
+    }
+    // printf("Exiting = %s\n", __myname);
+    return NULL;
+}
