AVATAR_executablecode/generated_src/EDRSystemBlock.h
@@ -15,15 +15,19 @@
 #include "tracemanager.h"
 #include "main.h"
 
+#include "ParseDoor.h"
+#include "ParseIndicator.h"
+#include "ParseSpeed.h"
+
 extern void *mainFunc__EDRSystemBlock(void *arg);
 __attribute__((unused)) request __req0__EDRSystemBlock;
-__attribute__((unused))int *__params0__EDRSystemBlock[0];
+__attribute__((unused)) int *__params0__EDRSystemBlock[0];
 __attribute__((unused)) request __req1__EDRSystemBlock;
-__attribute__((unused))int *__params1__EDRSystemBlock[0];
+__attribute__((unused)) int *__params1__EDRSystemBlock[0];
 __attribute__((unused)) request __req2__EDRSystemBlock;
-__attribute__((unused))int *__params2__EDRSystemBlock[0];
-__attribute__((unused))setOfRequests __list__EDRSystemBlock;
-__attribute__((unused))pthread_cond_t __myCond__EDRSystemBlock;
-__attribute__((unused))request *__returnRequest__EDRSystemBlock;
+__attribute__((unused)) int *__params2__EDRSystemBlock[0];
+__attribute__((unused)) setOfRequests __list__EDRSystemBlock;
+__attribute__((unused)) pthread_cond_t __myCond__EDRSystemBlock;
+__attribute__((unused)) request *__returnRequest__EDRSystemBlock;
 
 #endif
