AVATAR_executablecode/generated_src/main.c
@@ -18,33 +18,32 @@ pthread_mutex_t __mainMutex;
 
 #include "EDRSystemBlock.h"
 
+int main(int argc, char *argv[])
+{
 
-int main(int argc, char *argv[]) {
-  
-  /* disable buffering on stdout */
-  setvbuf(stdout, NULL, _IONBF, 0);
-  
-  /* Synchronous channels */
-  /* Asynchronous channels */
-  
-  /* Threads of tasks */
-  pthread_t thread__EDRSystemBlock;
-  /* Activating tracing  */
-  /* Activating randomness */
-  initRandom();
-  /* Initializing the main mutex */
-if (pthread_mutex_init(&__mainMutex, NULL) < 0) { exit(-1);}
-  
-  /* Initializing mutex of messages */
-  initMessages();
-  
-  
-  pthread_create(&thread__EDRSystemBlock, NULL, mainFunc__EDRSystemBlock, (void *)"EDRSystemBlock");
-  
-  
-  pthread_join(thread__EDRSystemBlock, NULL);
-  
-  
-  return 0;
-  
+    /* disable buffering on stdout */
+    setvbuf(stdout, NULL, _IONBF, 0);
+
+    /* Synchronous channels */
+    /* Asynchronous channels */
+
+    /* Threads of tasks */
+    pthread_t thread__EDRSystemBlock;
+    /* Activating tracing  */
+    /* Activating randomness */
+    initRandom();
+    /* Initializing the main mutex */
+    if (pthread_mutex_init(&__mainMutex, NULL) < 0)
+    {
+        exit(-1);
+    }
+
+    /* Initializing mutex of messages */
+    initMessages();
+
+    pthread_create(&thread__EDRSystemBlock, NULL, mainFunc__EDRSystemBlock, (void *)"EDRSystemBlock");
+
+    pthread_join(thread__EDRSystemBlock, NULL);
+
+    return 0;
 }
